Arithmetic/theories/Theorems.v
@@ -1,5 +1,5 @@
 From Coq Require Import ZArith.ZArith Strings.String.
-From RAC Require Import Utils Environnement Macros.
+From RAC Require Import Utils Environnement Macros Oracle Translation.
 From RAC.Languages Require Import Syntax Semantics.
 
 Open Scope utils_scope.
@@ -7,48 +7,132 @@ Open Scope utils_scope.
 From RecordUpdate Require Import RecordUpdate.
 Import RecordSetNotations.
 
-
-(* Proofs of structural properties of the translation *)
-
-Lemma mpz_pointer_invariant : True. 
-Proof.
-auto.
-Qed.
-
-Lemma absence_of_aliasing : 
-    forall (* program...*) z, type_of_value (Some z) = Some (T_Ext Mpz) -> True.
-auto.
-Qed.
+Module Theorems(Oracle:Oracle).
+    
+    Module T := Translation(Oracle).
 
 
-(* Theorem absence_of_dangling_pointers :
-    forall n (z:=VMpz n) (mem_state:𝓜) (var_env:Ωᵥ), 
-        mem_state n <> ⊥ n <-> 
-        exists x, var_env x = Some z /\
-        ~(exists x', x <> x' -> var_env x <> Some z)
+    (* Section C : PROPERTIES OF THE SEMANTICS *)
+    (* -> Languages/{MiniC,MiniGMP}/Lemmas.v *)
+
+
+
+
+    (* Section D : PROOFS OF STRUCTURAL PROPERTIES OF THE TRANSLATION *)
+
+    Lemma LD1_mpz_pointer_invariant : forall P args env env',
+        (gmp_pgrm_sem env (T.translate_program P) args env')  -> True.
+    Proof.
+    auto.
+    Qed.
+
+    Lemma LD2_absence_of_aliasing : True.
+    Proof.
+        auto.
+    Qed.
+
+    Lemma LD3_preservation_of_control_flow : True.
+    Proof.
+        auto.
+    Qed.
+
+    Lemma LD4 : True.
+    Proof.
+        auto.
+    Qed.
+
+
+    Lemma LD5_memory_transparency_of_generated_code : True.
+    Proof.
+        auto.
+    Qed.
+
+    Theorem T61_absence_of_dangling_pointers : True. 
+    Proof. 
+        auto.
+    Qed.
+
+
+    Theorem T62_absence_of_memory_leak : True. 
+    Proof. 
+        auto.
+    Qed.
+
+
+    (* Section E : PROOFS OF THE SEMANTICS OF THE MACROS *)
+
+    (* -> Macros.v *)
+
+    (* Section F  : INVARIANTS FOR ROUTINE TRANSLATION *)
+
+    (*
+
+    (* synchronicity invariant *)
+    Definition I1 (env:Ω) (ienv:Γ) := ((dom env.(binds)) = (dom (fst ienv) + dom (snd ienv)))%utils.
+
+    (* suitability invariant *)
+    Definition I2 (env:ψ) := True. (* todo *)
+
+    *)
+
+
+
+(*
+
+Inductive pgrm_var_representation (iop:ϴ) (e : Env) (ienv:Γ) : Env -> Prop :=
+| empty ΩΓ 𝓜Γ :   
+    I1 e ienv ->
+    let A := nil  (* { (iop ((snd ienv) v), v, (snd env) v ) | v in dom ienv  } *)
+    in
+    add_var_𝐴 e A {|env:=ΩΓ; mstate:=𝓜Γ|} -> 
+    pgrm_var_representation iop e ienv{|env:=ΩΓ; mstate:=𝓜Γ|}
 .
-Admitted. *)
+
+(* Definition well_formed_program :=
+    - all variables declared before usage
+    - all functions defined before called
+    - well typed
+*)
 
 
-(* Preservation of the semantics *)
+*)
 
-Open Scope fsl_sem_scope.
 
-(* Lemma semantics_of_term_translation : 
-    forall (t:fsl_term) Ω Γ Ψ z, 
-    I1 Ω Γ -> I2 Ψ ->
-    (Ω |= t => z <-> True)
-    .
-Proof.
-    intros. split.
-    - induction t eqn:T ; intro Hi.
-        * admit.
-        * admit.
-        * admit.
-        * admit.
-    - induction t eqn:T; intro Hi.
-        * admit.
-        * admit.
-        * admit.
-        * admit.
-Admitted. *)
+
+    (* Section G : PRESERVATION OF THE SEMANTICS *)
+
+    Open Scope fsl_sem_scope.
+
+    (*
+    Lemma LG1_semantics_of_term_translation : 
+        True
+    with LG2_semantics_of_predicate_translation : 
+        True
+    with LG3 : 
+        True.
+    Proof. 
+        auto.
+    Qed.
+    *)
+
+
+    Theorem TG4_soundness_of_assertion_translation : True.
+    Proof. 
+        auto.
+    Qed.
+
+
+    Theorem T64_correctness_of_code_generation :  forall (P:fsl_pgrm) args,
+
+        exists  (e  e' : Ω),
+        (fsl_pgrm_sem empty_env P args (empty_env <|env ; vars := e|>)
+        <-> 
+        gmp_pgrm_sem empty_env (T.translate_program P) args (empty_env <|env ; vars := e'|>)
+        )
+        /\ (e ⊑ e')%env.
+
+    Proof.
+    Admitted.
+
+
+End Theorems.
